doc/coq/simple/Sound.v
@@ -1,18 +1,17 @@
 From Simple Require Export Equiv.
-
-Module Abs := Abstract.
-Module Conc := Concrete.
+From Simple Require Export ALinking.
+From Simple Require Export Linking.
 
 Generalizable Variables CT AT.
 
-Definition preserve_tick `{Conc.time CT} `{Abs.time AT} (α : CT -> AT) :=
+Definition preserve_tick `{Concrete.time CT} `{Abstract.time AT} (α : CT -> AT) :=
   forall C m t x v,
   let abs_C := trans_C α C in
   let abs_m := trans_m α m in
   let abs_t := α t in
   let abs_v := trans_v α v in
-  α (Conc.tick C m t x v) = 
-    Abs.tick abs_C abs_m abs_t x abs_v.
+  α (Concrete.tick C m t x v) = 
+    Abstract.tick abs_C abs_m abs_t x abs_v.
 
 Ltac gen_leb :=
   match goal with
@@ -38,7 +37,7 @@ Ltac solve_leb tac :=
   | _ => tac
   end.
 
-Lemma sound_eval `{Conc.time CT} `{Abs.time AT} (α : CT -> AT) (PRES : preserve_tick α) :
+Theorem sound_eval `{Concrete.time CT} `{Abstract.time AT} (α : CT -> AT) (PRES : preserve_tick α) :
   forall e C m t ρ (EVAL : {|(Cf e C m t) ~> ρ|})
     (BOUND : time_bound_ρ (Cf e C m t)),
   let abs_C := trans_C α C in
@@ -106,4 +105,209 @@ Proof.
   end;
   gen_leb;
   solve_leb idtac.
+Qed.
+
+Generalizable Variables BCT BAT ACT AAT.
+
+Definition link_abs 
+  `{Concrete.time BCT} `{Abstract.time BAT} 
+  `{Concrete.time ACT} `{Abstract.time AAT}
+  (αbf : BCT -> BAT) (αaf : ACT -> AAT) :=
+  fun t : link BCT ACT =>
+  match t with
+  | BF t => BF (αbf t)
+  | AF t => AF (αaf t)
+  end.
+
+Lemma trans_ctx_lift
+  `{Concrete.time BCT} `{Abstract.time BAT}
+  `{Concrete.time ACT} `{Abstract.time AAT}
+  (αbf : BCT -> BAT) (αaf : ACT -> AAT) :
+  let αlink := (link_abs αbf αaf) in
+  forall C,
+    trans_C αlink (lift_ctx_bf C) =
+    lift_ctx_bf (trans_C αbf C).
+Proof.
+  induction C; simpl; repeat rw; eauto.
+Qed.
+
+Lemma trans_ctx_filter
+  `{Concrete.time BCT} `{Abstract.time BAT}
+  `{Concrete.time ACT} `{Abstract.time AAT}
+  (αbf : BCT -> BAT) (αaf : ACT -> AAT) :
+  forall C,
+  let αlink := (link_abs αbf αaf) in
+  trans_C αaf (filter_ctx_af C) = filter_ctx_af (trans_C αlink C).
+Proof.
+  induction C; simpl; repeat des_goal; repeat des_hyp;
+  clarify; repeat rw; eauto.
+Qed.
+
+Lemma trans_ctx_filter_bf
+  `{Concrete.time BCT} `{Abstract.time BAT}
+  `{Concrete.time ACT} `{Abstract.time AAT}
+  (αbf : BCT -> BAT) (αaf : ACT -> AAT) :
+  forall C,
+  let αlink := (link_abs αbf αaf) in
+  trans_C αbf (filter_ctx_bf C) = filter_ctx_bf (trans_C αlink C).
+Proof.
+  induction C; simpl; repeat des_goal; repeat des_hyp;
+  clarify; repeat rw; eauto.
+Qed.
+
+Lemma trans_ctx_link
+  `{Concrete.time BCT} `{Abstract.time BAT}
+  `{Concrete.time ACT} `{Abstract.time AAT}
+  (Cout : dy_ctx BCT) (αbf : BCT -> BAT) (αaf : ACT -> AAT) :
+  forall C,
+  let αlink := (link_abs αbf αaf) in
+  let eqb' t t' := eqb (αlink t) (αlink t') in
+  trans_C αaf
+    (filter_ctx_af (delete eqb' (lift_ctx_bf Cout) C)) =
+  filter_ctx_af
+    (delete eqb (lift_ctx_bf (trans_C αbf Cout)) (trans_C αlink C)).
+Proof.
+  intros.
+  rewrite <- trans_ctx_lift with (αbf := αbf) (αaf := αaf).
+  rewrite <- trans_C_delete.
+  rewrite trans_ctx_filter with (αbf := αbf) (αaf := αaf).
+  eauto.
+Qed.
+
+Lemma trans_m_aux_link
+  `{Concrete.time BCT} `{Abstract.time BAT}
+  `{Concrete.time ACT} `{Abstract.time AAT}
+  (Cout : dy_ctx BCT) (αbf : BCT -> BAT) (αaf : ACT -> AAT) :
+  forall (m : memory (link BCT ACT)) seen seen'
+    (EQ: forall t, In t seen <-> In (AF t) seen'),
+  let αlink := (link_abs αbf αaf) in
+  let eqb' t t' := eqb (αlink t) (αlink t') in
+  trans_m_aux αaf (filter_mem_af
+     (delete_ctx_mem eqb' (lift_ctx_bf Cout) m)) seen =
+  filter_mem_af
+     (delete_ctx_mem eqb (lift_ctx_bf (trans_C αbf Cout))
+        (trans_m_aux αlink m seen')).
+Proof.
+  induction m; ii; ss; repeat des_goal; repeat des_hyp; clarify; ss.
+  - erewrite IHm; eauto.
+  - erewrite IHm; eauto.
+    ii; ss; split; ii; des; clarify. 
+    right. rewrite EQ in *. eauto. 
+    rewrite <- EQ in *. eauto.
+  - erewrite IHm; eauto.
+  - rewrite Inb_eq in *.
+    rewrite Inb_neq in *.
+    rewrite EQ in *. contradict.
+  - rewrite Inb_eq in *.
+    rewrite Inb_neq in *.
+    rewrite <- EQ in *. contradict.
+  - rewrite IHm with (seen' := AF t :: seen').
+    destruct e; simpl.
+    rewrite trans_ctx_filter with (αbf := αbf) (αaf := αaf).
+    subst eqb'.
+    subst αlink.
+    pose proof (@trans_C_delete (link BCT ACT) (link BAT AAT) _ _) as RR.
+    rewrite RR.
+    rewrite trans_ctx_lift. eauto.
+    ii; split; ii; ss; des; clarify; eauto.
+    rewrite EQ in *. eauto.
+    rewrite <- EQ in *. eauto.
+Qed.
+
+Lemma trans_m_aux_link_bf
+  `{Concrete.time BCT} `{Abstract.time BAT}
+  `{Concrete.time ACT} `{Abstract.time AAT}
+  (αbf : BCT -> BAT) (αaf : ACT -> AAT) :
+  forall (m : memory (link BCT ACT))  seen seen'
+    (EQ: forall t, In t seen <-> In (BF t) seen'),
+  trans_m_aux αbf (filter_mem_bf m) seen =
+    filter_mem_bf (trans_m_aux (link_abs αbf αaf) m seen').
+Proof.
+  induction m; ii; ss; repeat des_goal; repeat des_hyp; clarify; ss.
+  - erewrite IHm; eauto.
+  - rewrite Inb_eq in *.
+    rewrite Inb_neq in *.
+    rewrite EQ in *. contradict.
+  - rewrite Inb_eq in *.
+    rewrite Inb_neq in *.
+    rewrite EQ in *. contradict.
+  - rewrite IHm with (seen' := BF t :: seen').
+    destruct e; simpl.
+    rewrite trans_ctx_filter_bf with (αbf := αbf) (αaf := αaf).
+    reflexivity.
+    ii; split; ii; ss; des; clarify; eauto.
+    rewrite EQ in *. eauto.
+    rewrite <- EQ in *. eauto.
+  - erewrite IHm; eauto.
+  - erewrite IHm; eauto.
+    ii; split; ii; ss; des; clarify; eauto.
+    rewrite EQ in *. eauto.
+    rewrite <- EQ in *. eauto.
+Qed.
+
+Lemma trans_m_link
+  `{Concrete.time BCT} `{Abstract.time BAT}
+  `{Concrete.time ACT} `{Abstract.time AAT}
+  (Cout : dy_ctx BCT) (αbf : BCT -> BAT) (αaf : ACT -> AAT) :
+  forall (m : memory (link BCT ACT)),
+  let αlink := (link_abs αbf αaf) in
+  let eqb' t t' := eqb (αlink t) (αlink t') in
+  trans_m αaf (filter_mem_af
+    (delete_ctx_mem eqb' (lift_ctx_bf Cout) m)) =
+  filter_mem_af
+    (delete_ctx_mem eqb (lift_ctx_bf (trans_C αbf Cout))
+      (trans_m αlink m)).
+Proof.
+  unfold trans_m. ii.
+  apply trans_m_aux_link.
+  ss.
+Qed.
+
+Lemma trans_m_link_bf
+  `{Concrete.time BCT} `{Abstract.time BAT}
+  `{Concrete.time ACT} `{Abstract.time AAT}
+  (αbf : BCT -> BAT) (αaf : ACT -> AAT) :
+  forall (m : memory (link BCT ACT)),
+  trans_m αbf (filter_mem_bf m) = filter_mem_bf (trans_m (link_abs αbf αaf) m).
+Proof.
+  unfold trans_m. ii.
+  apply trans_m_aux_link_bf.
+  ss.
+Qed.
+
+Theorem link_abs_pres
+  `{Concrete.time BCT} `{Abstract.time BAT}
+  `{Concrete.time ACT} `{Abstract.time AAT}
+  (Cout : dy_ctx BCT) (αbf : BCT -> BAT) (αaf : ACT -> AAT)
+  (PRESb : preserve_tick αbf) (PRESa : preserve_tick αaf):
+  @preserve_tick
+    (link BCT ACT) _ _ (Linking.link_time Cout (link_abs αbf αaf))
+    (link BAT AAT) _ (ALinking.link_time (trans_C αbf Cout))
+    (link_abs αbf αaf).
+Proof.
+  unfold preserve_tick in *.
+  simpl Concrete.tick. simpl Abstract.tick.
+  ii; destruct t; ss; repeat des_goal; repeat des_hyp; clarify;
+  match goal with
+  | |- BF ?a = BF ?b =>
+    let RR := fresh "RR" in
+    assert (a = b) as RR;
+    first [rewrite RR; reflexivity | idtac]
+  | |- AF ?a = AF ?b =>
+    let RR := fresh "RR" in
+    assert (a = b) as RR;
+    first [rewrite RR; reflexivity | idtac]
+  end.
+  - rewrite PRESb.
+    destruct v. s.
+    repeat rewrite (trans_ctx_filter_bf αbf αaf).
+    rewrite (trans_m_link_bf αbf αaf). eauto.
+  - rewrite PRESa.
+    pose proof (trans_m_link Cout αbf αaf) as RR.
+    rewrite RR.
+    destruct v. s.
+    repeat rewrite (trans_ctx_filter αbf αaf).
+    pose proof (trans_C_delete (link_abs αbf αaf)) as RR'.
+    repeat rewrite RR'.
+    rewrite trans_ctx_lift. eauto.
 Qed.
